updates

high2/Zeta.High.Verifier.fst
@@ -4,3 +4,15 @@ let lemma_high_verifier (aprm: app_params)
   : Lemma (ensures (GV.clock_monotonic_prop (high_verifier_spec_base aprm) /\
                     GV.thread_id_constant_prop (high_verifier_spec_base aprm)))
   = admit()
+
+let runapp_doesnot_change_store_addmethod
+  (#app:_)
+  (ki: base_key)
+  (e: vlog_entry app {Zeta.GenericVerifier.RunApp? e})
+  (vs: vtls_t app)
+  : Lemma (ensures (let vs_post = Zeta.GenericVerifier.verify_step e vs in
+                    vs_post.valid ==>
+                    store_contains vs.st ki ==>
+                    store_contains vs_post.st ki /\
+                    add_method_of vs.st ki = add_method_of vs_post.st ki))
+  = admit()
