high2/Zeta.High.SeqConsistent.fst
@@ -1,0 +1,347 @@
+module Zeta.High.SeqConsistent
+
+let eac_value_snoc (#app #n:_) = Zeta.High.Merkle.eac_value_snoc_appkey #app #n
+
+let eac_app_state (#app #n:_) (il: eac_log app n) (ak: app_key app.adm)
+  = let gk = AppK ak in
+    AppV?.v (eac_value gk il)
+
+let eac_value_is_eac_state_value (#app #n:_) (il: eac_log app n) (ak: app_key app.adm)
+  : Lemma (ensures (let gk = AppK ak in
+                    let es = eac_state_of_genkey gk il in
+                    match es with
+                    | EACInStore _ _ gv -> eac_value gk il = gv
+                    | EACEvictedMerkle _ gv -> eac_value gk il = gv
+                    | EACEvictedBlum _ gv _ _ -> eac_value gk il = gv
+                    | EACInit -> eac_value gk il = init_value gk))
+  = let gk = AppK ak in
+    let bk = to_base_key gk in
+    let es = eac_state_of_genkey gk il in
+    match es with
+    | EACInit -> eac_value_init_state_is_init il gk
+    | EACInStore _ _ gv ->
+      eac_app_state_value_is_stored_value il gk;
+      eac_value_is_stored_value il gk (stored_tid bk il)
+    | _ -> eac_value_is_evicted_value il gk
+
+let to_fc (#app #n:_) (il: eac_log app n) (i: seq_index il {RunApp? (index il i)})
+  : appfn_call app
+  = let App (RunApp fid_c arg_c _) inp_c = mk_vlog_entry_ext il i in
+    { fid_c; arg_c ; inp_c }
+
+let eac_implies_appfn_success (#app #n:_) (il: eac_log app n) (i: seq_index il {RunApp? (index il i)})
+  : Lemma (ensures (correct (to_fc il i)))
+          [SMTPat (to_fc il i)]
+  = let open Zeta.BinTree in
+    eac_state_transition Root il i
+
+let eac_app_prop (#app #n:_) (il: eac_log app n)
+  = let fcrs = app_fcrs il in
+    let fcs = app_fcs fcrs in
+    (* the results are valid meaning the output corresponds to the input records *)
+    valid_call_result fcrs /\
+    (* the app state as recorded by eac values is the same as the simulation state *)
+    post_state fcs == eac_app_state il
+
+let eac_app_prop_empty (#app #n:_) (il: eac_log app n)
+  : Lemma (ensures (length il = 0 ==> eac_app_prop il))
+  = if length il = 0 then (
+      let fcrs = app_fcrs il in
+      let fcs = app_fcs fcrs in
+
+      (* app call sequence is empty *)
+      app_fcrs_empty il;
+      assert(S.length fcs = 0);
+
+      (* an empty call sequence is valid *)
+      empty_call_result_valid (app_fcrs il);
+
+      (* the app state per the simulator - the initial state where everything is null *)
+      let sta = post_state fcs in
+
+      (* the eac state of the keys *)
+      let ste = eac_app_state il in
+
+      let aux (ak:app_key app.adm)
+        : Lemma (ensures (ste ak = sta ak))
+        = lemma_init_value_null fcs ak;
+          let bk = to_base_key (AppK ak) in
+          eac_state_empty bk il;
+          eac_value_init (AppK ak) il
+      in
+      FStar.Classical.forall_intro aux;
+      assert(app_state_feq ste sta)
+    )
+
+let app_refs_is_log_entry_refs
+  (#app #n:_)
+  (il: eac_log app n)
+  (i: seq_index il)
+  (ak: app_key app.adm)
+  : Lemma (requires (RunApp? (index il i)))
+          (ensures (let gk = AppK ak in
+                    let bk = to_base_key gk in
+                    let fc = to_fc il i in
+                    let e = index il i in
+                    let RunApp _ _ ss = e in
+                    fc `refs` ak ==>
+                    e `refs_key` bk /\ index_mem bk ss = refkey_idx fc ak))
+  = let RunApp _ _ refkeys = index il i in
+
+    let fc = to_fc il i in
+    if fc `refs_comp` ak then
+      (* the param index of ak *)
+      let idx = refkey_idx fc ak in
+
+      (* the key at location idx - we don't bk' = bk yet *)
+      let bk' = S.index refkeys idx in
+
+      (* relate the eac states before and after i for key bk' - the solver figures out the rest ... *)
+      eac_state_transition bk' il i
+
+let log_entry_refs_is_app_refs
+  (#app #n:_)
+  (il: eac_log app n)
+  (i: seq_index il)
+  (ak: app_key app.adm)
+  : Lemma (requires (RunApp? (index il i)))
+          (ensures (let gk = AppK ak in
+                    let bk = to_base_key gk in
+                    let fc = to_fc il i in
+                    let e = index il i in
+                    let il' = prefix il i in
+                    let il'' = prefix il (i+1) in
+                    let RunApp _ _ ss = e in
+                    e `refs_key` bk ==>
+                    ~ (fc `refs` ak) ==>
+                    eac_state_of_genkey gk il' = EACInit /\
+                    eac_state_of_genkey gk il'' = EACInit))
+  = let gk = AppK ak in
+    let bk = to_base_key gk in
+    let e = index il i in
+    let RunApp _ _ refkeys = e in
+    let fc = to_fc il i in
+    eac_state_transition bk il i;
+
+    if e `refs_key` bk && not (fc `refs_comp` ak) then
+      let idx = index_mem bk refkeys in
+      let ak',av' = S.index fc.inp_c idx in
+      let es' = eac_state_of_key_pre bk il i in
+      match es' with
+      | EACInStore _ gk' _ ->
+        assert(AppK ak' = gk');
+        if ak' = ak then refs_witness fc ak idx
+
+let eac_app_state_key_snoc_refs_key
+  (#app #n:_)
+  (il: eac_log app n {length il > 0}) (ak: app_key app.adm)
+  : Lemma (requires (let i = length il - 1 in
+                     RunApp? (index il i) /\
+                     to_fc il i `refs` ak))
+          (ensures (let i = length il - 1 in
+                    eac_app_state il ak = write (to_fc il i) ak))
+  = let i = length il - 1 in
+    let gk = AppK ak in
+    let bk = to_base_key gk in
+    eac_state_snoc bk il;
+    app_refs_is_log_entry_refs il i ak;
+    eac_app_state_value_is_stored_value il gk;
+    eac_value_is_stored_value il gk (stored_tid bk il)
+
+let eac_app_state_key_snoc (#app #n:_) (il: eac_log app n {length il > 0}) (ak: app_key app.adm)
+  : Lemma (ensures (let i = length il - 1 in
+                    let e = index il i in
+                    let il' = prefix il i in
+                    match e with
+                    | RunApp f p ss ->
+                      let fc = to_fc il i in
+                      if fc `refs_comp` ak then
+                        eac_app_state il ak = write fc ak
+                      else
+                        eac_app_state il ak = eac_app_state il' ak
+                    | _ -> eac_app_state il ak = eac_app_state il' ak))
+  = let i = length il - 1 in
+    let e = index il i in
+    let ee = mk_vlog_entry_ext il i in
+    let il' = prefix il i in
+    let gk = AppK ak in
+    let bk = to_base_key gk in
+    eac_value_snoc gk il;
+    eac_state_snoc bk il;
+    SA.lemma_fullprefix_equal il;
+
+    match e with
+    | RunApp f p ss ->
+      app_refs_is_log_entry_refs il i ak;
+      log_entry_refs_is_app_refs il i ak;
+      let fc = to_fc il i in
+      if fc `refs_comp` ak then
+        eac_app_state_key_snoc_refs_key il ak
+      else if e `refs_key` bk then (
+        eac_value_init_state_is_init il gk;
+        eac_value_init_state_is_init il' gk
+      )
+    | _ -> ()
+
+let eac_app_state_nonapp_snoc (#app #n:_) (il: eac_log app n {length il > 0})
+  : Lemma (ensures (let i = length il - 1 in
+                    let il' = prefix il i in
+                    not (RunApp? (index il i)) ==>
+                    eac_app_state il == eac_app_state il'))
+  = let i = length il - 1 in
+    let il' = prefix il i in
+    let e = index il i in
+    if not (RunApp? e) then (
+      let aux (ak:_)
+        : Lemma (ensures (eac_app_state il ak = eac_app_state il' ak))
+        = eac_app_state_key_snoc il ak
+      in
+      FStar.Classical.forall_intro aux;
+      assert(app_state_feq (eac_app_state il) (eac_app_state il'))
+    )
+
+let eac_implies_input_consistent_key
+  (#app #n:_)
+  (il: eac_log app n)
+  (i: seq_index il)
+  (ak: app_key app.adm)
+  : Lemma (requires (RunApp? (index il i)))
+          (ensures (let il' = prefix il i in
+                    let fc = to_fc il i in
+                    let st = eac_app_state il' in
+                    fc `refs` ak ==>
+                    refkey_inp_val fc ak = st ak))
+  = let gk = AppK ak in
+    let bk = to_base_key gk in
+    let il' = prefix il i in
+    let fc = to_fc il i in
+    app_refs_is_log_entry_refs il i ak;
+    eac_state_transition bk il i;
+    if fc `refs_comp` ak then
+      eac_value_is_eac_state_value il' ak
+
+let eac_implies_input_consistent
+  (#app #n:_)
+  (il: eac_log app n)
+  (i: seq_index il)
+  : Lemma (requires (RunApp? (index il i)))
+          (ensures (let il' = prefix il i in
+                    let fc = to_fc il i in
+                    let st = eac_app_state il' in
+                    input_consistent fc st))
+  = let fc = to_fc il i in
+    let il' = prefix il i in
+    let st = eac_app_state il' in
+
+  let aux (ak: app_key app.adm)
+    : Lemma (ensures (fc `refs` ak ==> refkey_inp_val fc ak = st ak))
+    = eac_implies_input_consistent_key il i ak
+  in
+  FStar.Classical.forall_intro aux
+
+#push-options "--z3rlimit_factor 3"
+
+let eac_app_state_app_snoc (#app #n:_) (il: eac_log app n {length il > 0})
+  : Lemma (requires (let i = length il - 1  in
+                     let il' = prefix il i in
+                     RunApp? (index il i) /\ eac_app_prop il'))
+          (ensures (let fcs = app_fcs (app_fcrs il) in
+                    valid fcs /\
+                    eac_app_state il == post_state fcs))
+  = let i = length il - 1 in
+    let fcr = to_app_fcr il i in
+    let il' = prefix il i in
+
+    let fcrs = app_fcrs il in
+    let fcs = app_fcs fcrs in
+    let fcrs' = app_fcrs il' in
+    let fcs' = app_fcs fcrs' in
+    let fc = to_fc il i in
+
+    appfn_calls_snoc il;
+    ext_app_records_is_stored_val il i;
+    app_fcs_snoc fcrs;
+    SA.lemma_prefix1_append fcrs' fcr;
+    SA.lemma_prefix1_append fcs' fc;
+
+    let st' = post_state fcs' in
+    assert(st' == eac_app_state il');
+    eac_implies_input_consistent il i;
+    correct_succeeds_if_input_consistent fc st';
+    assert(valid fcs);
+
+    let sts = post_state fcs in
+    let ste = eac_app_state il in
+    let aux (ak: app_key app.adm)
+      : Lemma (ensures (sts ak = ste ak))
+      = app_refs_is_log_entry_refs il i ak;
+        lemma_post_state fc st' ak;
+        eac_app_state_key_snoc il ak
+    in
+    FStar.Classical.forall_intro aux;
+    assert(app_state_feq sts ste)
+
+#pop-options
+
+#push-options "--z3rlimit_factor 3"
+
+let eac_implies_app_prop_snoc (#app #n:_) (il: eac_log app n {length il > 0})
+  : Lemma (requires (let i = length il - 1 in
+                     let il' = prefix il i in
+                     eac_app_prop il'))
+          (ensures eac_app_prop il)
+  = let i = length il - 1 in
+    let il' = prefix il i in
+    let fcrs = app_fcrs il in
+    let fcs = app_fcs fcrs in
+    let fcrs' = app_fcrs il' in
+    let fcs' = app_fcs fcrs' in
+    let e = index il i in
+    appfn_calls_snoc il;
+    eac_app_state_nonapp_snoc il;
+
+    match e with
+    | RunApp f p ss ->
+      let fcr = to_app_fcr il i in
+      let fc = to_fc il i in
+      let st' = post_state fcs' in
+      eac_app_state_app_snoc il;
+      appfn_calls_snoc il;
+      SA.lemma_prefix1_append fcrs' fcr;
+      SA.lemma_prefix1_append fcs' fc;
+      ext_app_records_is_stored_val il i;
+      valid_call_result_snoc fcrs;
+      eac_implies_input_consistent il i;
+      correct_succeeds_if_input_consistent fc st'
+    | _ -> ()
+
+#pop-options
+
+let rec eac_implies_app_prop (#app #n:_) (il: eac_log app n)
+  : Lemma (ensures (eac_app_prop il))
+          (decreases (length il))
+  = eac_app_prop_empty il;
+    if length il > 0 then (
+      let i = length il - 1 in
+      let il' = prefix il i in
+      eac_implies_app_prop il';
+      eac_implies_app_prop_snoc il
+    )
+
+let interleaving_implies_interleave (#a #n:_) (il: interleaving a n)
+  : Lemma (ensures (interleave (i_seq il) (s_seq il)))
+  = let is = i_seq il in
+    let ss = s_seq il in
+    FStar.Classical.exists_intro (fun il -> i_seq il = is /\ s_seq il = ss) il
+
+let lemma_eac_implies_appfn_calls_seq_consistent (#app #n:_) (il: eac_log app n)
+  : Lemma (ensures (let gl = to_glog il in
+                    Zeta.AppSimulate.seq_consistent (G.app_fcrs gl)))
+  = let fcrs_il = app_fcrs_il il in
+    let fcrs = i_seq fcrs_il in
+    let fcrss = s_seq fcrs_il in
+    interleaving_implies_interleave fcrs_il;
+    assert(interleave fcrs fcrss);
+    eac_implies_app_prop il;
+    assert(valid_call_result fcrs);
+    FStar.Classical.exists_intro (fun is -> interleave #(appfn_call_res app) is fcrss) fcrs
